cleaner setup

theories/Linearity.v
@@ -17,6 +17,8 @@ CoInductive sgType  : Type :=
 Set Elimination Schemes.
 
 
+Search _ Forall.
+
 Inductive Forall2 (A B : Type) (R : A -> B -> Type) : seq A -> seq B -> Prop :=
     Forall2_nil : Forall2 R nil nil | Forall2_cons : forall (x : A) (y : B) (l : seq A) (l' : seq B), R x y -> Forall2 R l l' -> Forall2 R (x :: l) (y :: l').
 Hint Constructors Forall2. Search List.Forall.
@@ -24,6 +26,28 @@ Hint Constructors Forall2. Search List.Forall.
 Inductive Forall3 (A B C : Type) (R : A -> B -> C -> Type) : seq A -> seq B -> seq C -> Prop :=
     Forall3_nil : Forall3 R nil nil nil | Forall3_cons : forall (x : A) (y : B) (z : C) (l : seq A) (l' : seq B) (l'' : seq C), R x y z -> Forall3 R l l' l'' -> Forall3 R (x :: l) (y :: l') (z ::l'').
 Hint Constructors Forall3.
+
+Lemma index_Forall : forall (A: Type) (l0 : seq A) d0 n (P : A  -> Prop), n < size l0 -> Forall P l0 -> P (nth d0 l0 n).
+Proof.
+intros. move : H0 d0 n H. elim.
+intros.  done. intros. destruct n. simpl. done. simpl. auto. 
+Qed.
+
+
+Lemma size_Forall2 : forall (A B : Type) (l0 : seq A) (l1 : seq B) P, Forall2 P l0 l1 -> size l0 = size l1. 
+Proof. intros. induction H;simpl;auto. Qed.
+
+Lemma index_Forall2 : forall (A B : Type) (l0 : seq A) (l1 : seq B) d0 d1 n (P : A -> B -> Prop), n < size l0 -> Forall2 P l0 l1 -> P (nth d0 l0 n) (nth d1 l1 n).
+Proof.
+intros. move : H0 d0 d1 n H. elim.
+intros.  done. intros. destruct n. simpl. done. simpl. auto. 
+Qed.
+
+Lemma Forall2_Forall : forall (A B : Type) (l0 : seq A) (l1 : seq B) (P : A -> Prop), Forall2 (fun a b => P a) l0 l1 -> Forall P l0.
+Proof.
+intros. elim : H;auto.
+Qed.
+
 
 Inductive Unravel (r : gType -> sgType -> Prop) : gType -> sgType -> Prop :=
  | UEnd : Unravel r GEnd SGEnd
@@ -251,7 +275,7 @@ Canonical label_predType := PredType pred_of_label.
 Inductive Tr : seq action -> sgType -> Prop :=
 | TR_nil G : Tr nil G 
 | TRMsg a u aa g0 : Tr aa g0 -> Tr (a::aa) (SGMsg a u g0)
-| TRBranch a gs n aa : Tr aa (nth SGEnd gs n) ->  Tr (a::aa) (SGBranch a gs).
+| TRBranch a gs n aa d : n < size gs -> Tr aa (nth d gs n) ->  Tr (a::aa) (SGBranch a gs).
 Hint Constructors Tr.
 (*Fixpoint tr (ls : seq action) (sg : sgType)  {struct ls}  :=
 match sg,ls with 
@@ -273,13 +297,18 @@ Definition exists_depP  (Pm : seq bool -> Prop) (P : seq action -> Prop) a0 aa a
 Notation exists_dep := (exists_depP (fun _ => True)).
 
 
-Definition Linear (sg : sgType) := forall aa_p a0 aa a1, 
-Tr (aa_p ++ (a0::aa++[::a1])) sg -> 
+Definition Linear (sg : sgType) := forall s aa_p a0 aa a1, s = aa_p ++ (a0::(aa++[::a1])) -> 
+Tr s sg -> 
 same_ch a0 a1 -> 
 exists_dep InDep a0 aa a1 /\ exists_dep OutDep a0 aa a1.
-Print sum.
-Definition value_nat := (@sum value nat).
-Identity Coercion value_nat_coercion : value_nat >-> sum.
+
+Definition Linear1 (sg : sgType) := forall aa_p a0 aa a1, 
+Tr (aa_p ++ (a0::(aa++[::a1]))) sg -> 
+same_ch a0 a1 -> 
+exists_dep InDep a0 aa a1.
+
+(*Definition value_nat := (@sum value nat).
+Identity Coercion value_nat_coercion : value_nat >-> sum.*)
 
 (*FunClass coercion*)
 (*Parameter (c : ch) (p : ptcp). Check Action.
@@ -330,6 +359,334 @@ intros. apply H2;auto.
 intros. apply H3;auto. elim : f;auto.  
 Qed.
 
+
+(*Lemma step_tr_in : forall g vn g', step g vn g' -> forall s, Tr s g' -> Tr s g \/ exists s1 s2, s = s1++s2 /\ Tr (s1 ++ vn.1::s2) g /\ Forall (fun a => (ptcp_to a) \notin vn.1) s1.
+Proof.
+move => g vn g'. elim.
+- intros. right. exists nil,s. simpl. auto.  
+- intros. right. exists nil,s. simpl. split;auto.  split;auto.   eapply TRBranch with (n:=n). done. apply : H0. 
+- intros. destruct s;auto. 
+  inversion H2. subst. move : (H0 _ H4)=>[]. auto. move=> [] s1 [] s2 [] Heq [] Htr Hf. right. subst. exists (a::s1),s2. rewrite /=.  auto. 
+- intros. destruct s. auto.
+  inversion H2. subst. have :
+          forall (d0 d1 : sgType) s,
+          Tr s (nth d1 gs' n) -> Tr s (nth d0 gs n) \/ (exists s1 s2 : seq action, s = s1 ++ s2 /\ Tr (s1 ++ l.1 :: s2)  (nth d0 gs n) /\ Forall (fun a : action => ptcp_to a \notin l.1) s1).
+  move => d0 d1. apply index_Forall2 with (l0:=gs)(l1:=gs'). rewrite (size_Forall2 H0). done. done. intros.
+  case  : (x d d s H8). intros. left. apply : TRBranch. rewrite (size_Forall2 H0). apply : H6.  apply : a0. 
+  move => [] s1 [] s2 [] Heq [] Htr Hf. right. exists (a::s1),s2. subst. rewrite /=. split;auto. split;auto. apply : TRBranch.
+  rewrite (size_Forall2 H0). apply : H6. apply : Htr.
+Qed.
+Check InDep.*)
+
+Definition insert (A : Type) (l : seq A) n x := ((take n l) ++ (x::(drop n l))).
+
+Lemma insert0 : forall (A: Type) (l : seq A) x, insert l 0 x = x::l.
+Proof. intros. by rewrite /insert take0 drop0 /=. Qed.
+
+Lemma insert_nil : forall (A: Type) n (x : A), insert nil n x  = [::x]. 
+Proof. intros. destruct n; done. Qed.
+
+
+Lemma insert_cons : forall (A: Type) (l : seq A) n x a, insert (a::l) n x  = if n is n'.+1 then a::(insert l n' x) else x::a::l.
+Proof. intros. destruct n.  rewrite insert0. done. rewrite /insert /=. done. Qed.
+
+Lemma insert_cat : forall (A: Type) (l0 l1 : seq A) n x, insert (l0++l1) n x  = if n <= size l0 then (insert l0 n x)++l1 else l0++(insert l1 (n-(size l0)) x). 
+Proof. move => A.  elim. rewrite /=. intros. destruct n. by rewrite insert0 /=. rewrite /=. done. 
+intros. rewrite /=. rewrite insert_cons. destruct n. by rewrite /=. rewrite H /=. destruct (n < (size l).+1) eqn:Heqn. 
+have : n <= size l by lia.  move=>->. f_equal. have : n <= size l = false by lia. move=>->. done. 
+Qed.
+
+
+
+
+
+Lemma step_tr_in : forall g vn g', step g vn g' -> forall s, Tr s g' -> Tr s g \/ exists n, Tr (insert s n vn.1) g /\ Forall (fun a => (ptcp_to a) \notin vn.1) (take n s).
+Proof.
+move => g vn g'. rewrite /insert. elim.
+- intros. right. exists 0. simpl. rewrite take0 drop0 /=.  auto. 
+- intros. right. exists 0. simpl. rewrite take0 drop0 /=.  split;auto.  eauto. 
+- intros. destruct s;auto. 
+  inversion H2. subst. move : (H0 _ H4)=>[];auto.
+  move=> [] n [].  intros. right. exists n.+1. simpl. auto. 
+- intros. destruct s; auto.
+  inversion H2. subst. rewrite -(size_Forall2 H0) in H6.  
+  case :  (@index_Forall2 _ _ gs gs' d d n _ H6 H0 _ H8). 
+ * intros. left. eauto.
+ * move => [] n0 [] HH0 HH1. right. exists n0.+1. rewrite /=. eauto. 
+Qed.
+
+(*Lemma insert_split_tr : forall aa_0 a0 a_mid a1, insert (aa_0++(a0::(a_mid++[::a1]))) n x = 
+if x <= size aa_0 then (insert aa_0 n x)++(a0::(a_mid++[::a1]))
+else if x <= size (aa_0).+1 (size aa_0).+1 then aa_0 ++ x::a0::(a_mid++[::a1])
+else if *)
+
+(*Lemma tr_linear1 : forall s n x aa_p a0 s_mid a1, insert s n x = aa_p++(a0::(s_mid++[::a1])) -> exists_dep InDep a0 s_mid a1 -> *)
+
+Lemma Tr_app : forall l0 l1 G, Tr (l0++l1) G -> Tr l0 G.
+Proof.
+elim. rewrite /=. done.
+move => a l IH l1 G. rewrite cat_cons. move => H. inversion H. 
+- subst. constructor. eauto.  
+- subst. eauto. 
+Qed.
+
+Lemma linear1_step : forall g l g', step g l g' -> Linear1 g -> Linear1 g'.
+Proof.
+intros. rewrite /Linear1. intros. move : (step_tr_in H H1)=>[]. intros. eauto.  
+move => [] n [] Htr Hf. move : Htr. rewrite insert_cat.
+destruct (n <= size aa_p) eqn:Heqn;eauto. 
+rewrite insert_cons. destruct (n - size aa_p) eqn:Heqn2. 
+have : (aa_p ++ [:: l.1, a0 & aa ++ [:: a1]]) = ((aa_p ++ [:: l.1])++ a0::aa ++ [:: a1]). by rewrite -catA /=.
+move=>->. eauto. 
+rewrite insert_cat. destruct (n0 > size aa) eqn:Heqn3.
+have : n0 <= size aa = false by lia. move=>->. 
+rewrite insert_cons. destruct (n0 - size aa) eqn:Heqn4. lia. rewrite insert_nil.
+have : aa_p ++ a0 :: aa ++ [:: a1; l.1] = (aa_p ++ a0 :: aa ++ [:: a1]) ++ [::l.1]. rewrite -!catA !cat_cons. f_equal. Search _ (_ :: (_ ++ _)). f_equal. rewrite -catA. f_equal. move=>->. eauto. move/Tr_app. eauto. 
+have : n0 <= size aa by lia. move=>->. intros. (*setup finished*)
+move : (H0 _ _ _ _ Htr H2)=>Hlin.
+move : Hf. have : n = n0.+1 + (size aa_p) by lia. move=>->. rewrite take_cat.
+have :  n0.+1 + size aa_p < size aa_p = false by lia. move=>->. rewrite /=.
+have : (n0.+1 + size aa_p - size aa_p) = n0.+1  by lia. move=>->.
+rewrite /=. rewrite take_cat2. have : n0 < size aa by lia.
+rewrite cat_cons. f_equal. rewrite cat_cons.  catA. cat_cons.
+
+Search _ (_ ++ Check cons_cat.
+- rewrite -[aa_p ++ _]cat_cons.
+- 
+  intros. eauto. 
+- rewrite drop_ca
+Lemma split_list : forall A (l : seq A), l = nil \/ exists l' a, l = l'++([::a]).
+Proof.
+move => A. elim.
+auto.  move => a l [] . move =>->. right.  exists nil. exists a. done. 
+move => [] l' [] a0 ->. right. exists (a::l'). exists a0. done.
+Qed.
+
+
+
+Lemma last_eq : forall A (l0 l1 : seq A) x0 x1, l0 ++ ([::x0]) = l1 ++ ([::x1]) -> l0 = l1 /\ x0 = x1.
+Proof.
+move => A. elim.
+case. rewrite /=. move => x0 x1. case. done.
+move => a l x0 x1. rewrite /=. case. move =>-> H. apply List.app_cons_not_nil in H. done. 
+rewrite /=. intros. case : l1 H0.  rewrite /=. case. move => _ /esym H1. apply List.app_cons_not_nil in H1. done. 
+intros. move : H0.  rewrite cat_cons. case. intros. move : (H _ _ _ H1). case. intros. split. subst. done. done. 
+Qed.
+
+
+  
+
+Lemma split_mask : forall A (l0 : seq A) x l1 m, size m = size (l0++x::l1) ->
+mask m (rcons l0 x ++ l1) =
+  mask (take (size l0) m) l0 ++ (nseq (nth false m (size l0)) x) ++ mask (drop (size l0).+1 m) l1.
+Proof.
+move => A. elim. 
+- rewrite /=. intros. rewrite take0 /=. case : m H. done. 
+  intros. by  rewrite mask_cons /= drop0. 
+- rewrite /=. intros. case : m H0.  done. rewrite /=. intros. 
+  case : a0. rewrite cat_cons. f_equal. rewrite H //=. lia. 
+  rewrite H //=. lia.
+Qed.
+
+
+Lemma split_has_indep : forall s1 s2 l, Forall (fun a => (ptcp_to a) \notin l) s1 -> InDep (s1 ++ l::s2) -> InDep (s1 ++ s2).
+Proof. 
+Admitted.
+
+Lemma cons23 : forall A  s0 s1 aa (a0 : A) a1,  a0 :: aa ++ [:: a1] = s0 ++ s1 -> s0 = nil /\ a0::aa++([:: a1]) = s1 \/ s1 = nil /\  a0::aa++([:: a1]) = s0 \/ exists s0' s1', s0 = a0::s0' /\ s1 = s1'++([::a1]) /\ s0' ++ s1' =  aa.
+Proof.
+move => A. elim.
+move => s1 aa a0 a1. rewrite /=. move => <-. auto. 
+rewrite /=. intros. case : H0. move => <-. case : aa. rewrite /=. case : s1. rewrite cats0. move => <-. auto. 
+move => a2 l0. right. right. exists l. case : l H H0. rewrite /=. intros. exists nil. done. 
+rewrite /=. intros. case : H0.  intros. apply List.app_cons_not_nil in H1. done. 
+move => a2 l0. rewrite cat_cons. move/H. case. 
+- case. move => -> <-. right. right. exists nil. exists (a2::l0). done. 
+case. 
+ - case. move => -> <-. auto. 
+ - case.  move => x [] x1 [] -> [] -> H1. right. right. exists (a2::x). exists x1. rewrite /= H1. done. 
+Qed.
+
+Definition IO_II a0 a1 := IO a0 a1 || II a0 a1.
+
+Lemma indep0 : forall l0 l1, indep (l0 ++ l1) -> if l0 is x::l0' then path IO_II x l0' else true.
+Proof.
+move => l0 l1. rewrite /indep.
+case :l0 ;first done.
+move => a l. rewrite /=. case : l;first done.
+move => a0 l. rewrite /=. move/andP=> [] H H1. elim : l a a0 H H1.
+- move => a a0. rewrite /=.  case : l1. simpl. rewrite /IO_II. move => _ -> . by rewrite orbC.  
+  move => a1 l. rewrite/= /IO_II. by move/andP=> [] ->.
+- move => a l IH a0 a1. rewrite /= /IO_II. move/andP=> [] ->. intros. rewrite /=. 
+  unfold IO_II in IH. apply/IH. done. done.
+Qed.
+
+(*Lemma take_rcons : forall ( A: Type) l (a : A) n, n <= size l -> take n (rcons l a) = rcons (take n l) a.
+Proof.
+move => A. elim.
+- rewrite /=. move => a [].  rewrite take0.  done.*)
+
+(*Lemma IO_II_in : forall a0 (l : label), IO_II a0 l.1 -> a0 \in l.1.*)
+Lemma in_action_from' : forall p0 p1 c, p0 \in Action p0 p1 c.
+Proof. intros. by rewrite /in_mem /= eqxx. Qed.
+
+Lemma in_action_to' : forall p0 p1 c, p1 \in Action p0 p1 c.
+Proof. intros. by rewrite /in_mem /= orbC eqxx. Qed.
+
+Lemma in_action_from : forall a, ptcp_from a \in a.
+Proof. intros. destruct a. rewrite /=. rewrite in_action_from' //=. Qed.
+
+Lemma in_action_to : forall a, ptcp_to a \in a.
+Proof. intros. destruct a. rewrite /=. rewrite in_action_to' //=. Qed.
+
+Hint Resolve in_action_from in_action_to in_action_from' in_action_to'.
+
+Lemma IO_II_in_action : forall a0 (l : label), IO_II a0 l -> (ptcp_to a0) \in l.
+Proof.
+move => a0 a1. rewrite /IO_II. move/orP=>[]. rewrite /IO. move/eqP=>->. apply in_action_from.
+rewrite /II.  move/eqP=>->. apply in_action_to. 
+Qed.
+
+Lemma get_neigbor : forall (P : action -> action -> bool) a p x_end m, path P a (rcons (mask m p) x_end) -> exists x_in, x_in \in (a::p) /\ P x_in x_end. 
+Proof. 
+intros. 
+case : (split_list (mask m p)) H. move =>->. rewrite /= andbC /=. intros. exists a. by rewrite inE eqxx /=.
+move => [] l' [] a0 Heqa2.  move : (Heqa2) =>->. rewrite rcons_cat.  rewrite cat_path /=.
+move/andP=> [] _ /andP => [] [] _. rewrite andbC /=. move => HH.
+have : a0 \in a::p. rewrite inE.  apply/orP. right. apply (@mem_mask _ _  m). 
+rewrite Heqa2. by rewrite mem_cat inE eqxx orbC. 
+intros. exists a0. by rewrite x. 
+Qed.
+Search _ (Forall _ _).
+(*Lemma Forall_in : forall (A : eqType) (a : A) (l : seq A) (P : a -> Prop),  Forall P l. -> a \in l -> P a.
+Proof.
+move => A a. elim. done.
+intros. move : H1. rewrite inE. move/orP. case. move/eqP=>->. inversion H0. done. inversion H0. intros.   apply H. done. done.
+Qed. *)
+
+
+Lemma In_in : forall (A : eqType) (a : A) l, In a l <-> a \in l.
+Proof.
+move => A a. elim. split;done.
+intros. rewrite /= inE. split. case. move=>->. rewrite eqxx. done. move/H. move=>->. by rewrite orbC. 
+move/orP. case. move/eqP. move=>->. auto. move/H. auto. 
+Qed.
+
+
+Lemma delete_middle : forall a0 l0 a l1 a1 P, exists_depP (fun m => nth false m (size l0) = false) P a0 (rcons l0 a ++l1) a1 ->
+                      exists_dep P a0 (l0++l1) a1.
+Proof.
+intros. move : H => [] m [] H0 [] H1 H2. exists ((take (size l0) m)++(drop (size l0).+1 m)).
+rewrite size_cat size_take size_drop H0 !size_cat /=. have : size l0 <( size l0).+1 + (size l1) by lia.
+move => H3. rewrite size_rcons /=. rewrite H3. split. lia. split;auto. move : H1. rewrite !split_mask //=. rewrite H2 /= mask_cat //=. 
+by rewrite size_take  H0 size_cat /= size_rcons H3.  rewrite H0 size_cat size_rcons /= size_cat /=.  lia. 
+Qed.
+
+Lemma take_rcons : forall (A : Type) l n (a : A), n <= size l -> take n (rcons l a) = take n l.
+Proof.
+move => A. elim.
+case;try done. simpl. intros. rewrite take_cons. case : n H0. by rewrite take0.
+intros. simpl. f_equal. auto. 
+Qed.
+
+
+Lemma linear_step : forall g l g', step g l g' -> Linear g -> Linear g'.
+Proof.
+intros. rewrite /Linear. intros. move : (step_tr_in2 H H1)=>[]. intros. eauto.  
+move => [] n [] Htr Hf. move : Htr. destruct (n < size aa_p) eqn:Heqn. 
+- rewrite drop_cat Heqn. rewrite -cat_rcons catA.
+  intros. eauto. 
+- rewrite drop_cat take_cat Heqn.
+  destruct ( n - size aa_p) eqn:Heqn2. rewrite take0 drop0 cats0 -cat_rcons.  intros. eauto. 
+  rewrite /=. Search _ drop. destruct (n0 <= size aa) eqn:Heqn3.
+ *  rewrite drop_rcons //=. rewrite -rcons_cons. rewrite -cat_rcons -catA. rewrite -rcons_cat.  
+     rewrite cat_rcons. intros. apply H0 in Htr. apply Htr in H2. clear Htr.  destruct H2. split.
+  ** move : H2 => [] m [] Hsize [] Hin _. Search _ take.  (*InDep*)
+      case Heqb : (nth false m (size (take n0 (rcons aa a1)))).  
+
+      move : Hin. rewrite -[_ ++ l.1 ::_]cat_rcons. rewrite split_mask.  rewrite Heqb /=.
+      move/InDep_iff. rewrite -[_ ++ l.1::_]cat_rcons. rewrite -[_++a1::_]cat_rcons cats0. rewrite rcons_cat.
+      rewrite -cat_cons.  move/indep0. move : Hf. rewrite take_cat Heqn Heqn2 /=. 
+      rewrite size_take.  simpl. rewrite size_rcons. have : n0 < (size aa).+1 by lia.  move=>->.
+      move/List.Forall_app=>[ HH0 HH1]. inversion HH1.  subst. move/get_neigbor=>[] xin []. rewrite inE. move/orP. case.
+
+      move/eqP=>->.  move/IO_II_in_action=> Hin. by rewrite Hin in H5. 
+      
+intros. move : H6. move/List.Forall_forall=> HH. specialize HH with xin.  apply In_in in b. apply HH in b. 
+      apply IO_II_in_action in b0.  rewrite b0 in b. done.
+
+      rewrite Hsize. 
+
+
+      rewrite size_cat size_take size_rcons. have : n0 < (size aa).+1 by lia. move => Hn0. rewrite Hn0. rewrite /= size_drop //=.
+
+
+move : Hin Heqb Hsize. rewrite take_rcons //=. intros. rewrite size_take. intros.
+     
+      rewrite take_rcons in Hin. 
+
+
+rewrite -[aa](cat_take_drop n0). have : n0 < (size aa).+1 by lia. move => Hn0.
+     Search _ (take _ (rcons _ _)). 
+
+  apply : delete_middle. exists m. rewrite Hsize.  rewrite !size_cat !size_take size_rcons Hn0 /=. split. destruct (eqVneq n0 (size aa)). rewrite size_rcons size_take e ltnn size_drop.  lia. rewrite size_rcons size_take. have : n0 < size aa = true by lia. move=>->. lia. 
+       split.  
+
+
+(*Got to here*) 
+
+Search _ (_ != _ -> _ < _). by lia. e ltnn. lia. 
+   have : n0 < size aa by lia. move=>->. lia. split. apply : Hin. !size_drop. size_take size_rcons Hn0 size_cat size_take/=. split. destruct (eqVneq n0 (size aa)).  rewrite e. Search _ (?a < ?a).  rewrite ltnn. rewrite e in Hn0. done. lia. == size aa) eqn :Heqnn.  lia. lia. size_take size_drop. apply : delete_middle. 
+
+exists ((take n0 (rcons aa a1) ++ l.1 :: drop n0 aa)).
+rewrite split_mask in Hin. 
+
+      move : Hin. rewrite split_mask. rewrite Heqb /=. intros. exists ((take (size (take n0 (rcons aa a1))) m)++((drop (size (take n0 (rcons aa a1))).+1 m))). rewrite size_take /= size_rcons.  have : n0 < (size aa).+1 by lia. move => Hn0. rewrite Hn0. 
+      
+      rewrite size_cat size_take size_drop Hsize.  rewrite size_cat size_take size_rcons /= Hn0 size_drop. 
+      have : n0 < n0 + (size aa - n0).+1 by lia. move=>->. split. lia. split;auto.
+  rewrite b in b'. rewrite H5 in b. . eapply -> List.Forall_forall in H6.  have : xin \notin take n0 (rcons aa a1). eapply Forall_in.  apply : H6. _  H6). . 2 : { b0 H6).  apply List.Forall_app in Hf as [Hf0 Hf1]. inversion Hf1.
+      destruct (split_list (mask (take n0 m) (take n0 (rcons aa a1)))). rewrite H2. 
+      rewrite /= andbC /=. move =>  Hf Hio. 
+      apply IO_II_in_action in Hio. rewrite Hio in H6. done. 
+      destruct H2,H2. rewrite H2. move => Hf. rewrite rcons_cat. move/get_neigbor. rewrite cat_path. move/andP. rewrite /=. case. move => _. move/andP => [] _. move /andP => []. intros. Check mem_mask. move => path_rcons.  move => HH Hp.  intros.
+
+ Search _ mask. rewrite take_oversize //=. apply indep0 in HH.
+      intros.  move/indep0. rewrite indep0.
+     intros.
+
+
+
+//=. rewrite last (apply : delete_middle; exists m; split;eauto). 
+      move : Hin. rewrite split_mask //= Heqb /=.
+
+
+      move/InDep_iff.
+      have : (a :: (mask (take (size s0') m) s0' ++ l.1 :: mask (drop (size s0').+1 m) s1') ++ [:: a1]) =
+             (((a :: (mask (take (size s0') m) s0' ++ [::l.1])) ++ (mask (drop (size s0').+1 m) s1') ++ [:: a1])).
+      by rewrite /= -!catA. move =>->.
+
+      move/indep0. move/get_neigbor=> [] x_in []. intros.
+
+      exfalso. apply/negP. eapply reduce_condition with (a':=x_in). apply : Hstep.   apply : HG0. 
+      by rewrite mem_cat a0 orbC. apply IO_II_in_action. done. 
+rewrite -cat_cons. rewrite -!catA. rewrite -cat_cons.  rewrite -catA -rcons_cat.
+ * 2 : { rewrite drop_oversize.  rewrite take_oversize. intros. apply Tr_app in Htr. eauto. 
+     rewrite size_rcons.  lia. rewrite size_rcons. lia. lia. }
+    Search _ drop.
+have : aa_p ++ [:: l.1, a0 & aa ++ [:: a1]] =
+       (rcons aa_p l.1) ++ ((a0 :: aa) ++ [:: a1]).  -cat_cons.
+intros.
+
+ (aa_p ++ a0 :: aa ++ [:: a1]) ++ l.1 :: drop n aa_p ++ a0 :: aa ++ [:: a1] = 
+         ((aa_p ++ a0 :: aa ++ [:: a1]) ++ l.1 :: drop n aa_p) ++ a0 :: aa ++ [:: a1].
+  rewrite -!catA /=. done. intros. subst. rewrite x in Htr. move =>->. -!cat_cons /=.
+
+ rewrite drop_cat in Htr. rewrite Heqn inrewrite /Linear in H0. destruct s1. simpl in * . subst. rewrite -cat_cons in Htr. 
+apply : H0. apply : Htr. done. move : (@H0 _ _ _ _ Htr). apply H0 in Htr.  subst. destruct aa_p.  simpl in *.  apply : H0. subst. rewrite Heq. 
+2 : { rewrite -cat_cons in Heq. move : (cons23 Heq).  apply : H0. move : H. move/step_tr_in=> H.  in H.
+intros. case : (split_list s1).
+-intros. subst. simpl in H0.
 
 Unset Elimination Schemes. 
 Inductive stepG : sgType -> sgType -> label  -> sgType -> Prop :=
@@ -546,13 +903,7 @@ auto.  move => a l [] . move =>->. right.  exists nil. exists a. done.
 move => [] l' [] a0 ->. right. exists (a::l'). exists a0. done.
 Qed.
 
-Lemma Tr_app : forall l0 l1 G, Tr (l0++l1) G -> Tr l0 G.
-Proof.
-elim. rewrite /=. done.
-move => a l IH l1 G. rewrite cat_cons. move => H. inversion H. 
-- subst. constructor. eauto.  
-- subst. apply TRBranch with (n:=n). eauto.
-Qed.
+
 
 Lemma last_eq : forall A (l0 l1 : seq A) x0 x1, l0 ++ ([::x0]) = l1 ++ ([::x1]) -> l0 = l1 /\ x0 = x1.
 Proof.
@@ -578,6 +929,8 @@ move => A. elim.
   rewrite H //=. lia.
 Qed.
 
+
+(*copied until herew*)
 Lemma add_sub : forall n1 n0, n0 = n0 + n1 - n1. 
 elim.
 lia. 
@@ -611,15 +964,7 @@ elim. auto. rewrite /=. intros. apply H. inversion H0. subst. case : l H3 H0 H. 
 rewrite /=. intros. case : H3. intros. apply List.app_cons_not_nil in H3. done. done.
 Qed.
 
-Lemma in_action_to : forall a, in_action (ptcp_to a) a.
-Proof.
-case. intros. by rewrite/= eqxx orbC.
-Qed. 
 
-Lemma in_action_from : forall a, in_action (ptcp_from a) a.
-Proof.
-case. intros. by rewrite/= eqxx.
-Qed. 
 
 Lemma cons23 : forall A  s0 s1 aa (a0 : A) a1,  a0 :: aa ++ [:: a1] = s0 ++ s1 -> s0 = nil /\ a0::aa++([:: a1]) = s1 \/ s1 = nil /\  a0::aa++([:: a1]) = s0 \/ exists s0' s1', s0 = a0::s0' /\ s1 = s1'++([::a1]) /\ s0' ++ s1' =  aa.
 Proof.
@@ -636,16 +981,8 @@ case.
 Qed.
 
 
-Lemma InDep_app : forall l0 l1, InDep (l0 ++ l1) -> 1 < size l1 -> InDep l1.
-Proof.
-elim. rewrite /=. done.
-move => a l IH l1. rewrite cat_cons. move => H. inversion H. subst.
-case : l H2 H IH.  rewrite /=. move => <-. done. 
-move => a0 l. rewrite cat_cons. case. move => <-. case : l.  case : l1. done. done. done. 
-intros. subst. rewrite H1 in H3. auto. 
-Qed.
 
-Definition IO_II a0 a1 := IO a0 a1 || II a0 a1.
+
 
 Lemma ind_aux : forall l a a0, path IO a (belast a0 l) -> II (last a (belast a0 l)) (last a0 l) -> IO_II a a0 && path IO_II a0 l.
 Proof.
@@ -655,17 +992,7 @@ Proof.
   unfold IO_II in IH. apply/IH. done. done. 
 Qed.
 
-Lemma indep0 : forall l0 l1, indep (l0 ++ l1) -> if l0 is x::l0' then path IO_II x l0' else true.
-Proof.
-move => l0 l1. rewrite /indep.
-case :l0 ;first done.
-move => a l. rewrite /=. case : l;first done.
-move => a0 l. rewrite /=. move/andP=> [] H H1. elim : l a a0 H H1.
-- move => a a0. rewrite /=.  case : l1. simpl. rewrite /IO_II. move => _ -> . by rewrite orbC.  
-  move => a1 l. rewrite/= /IO_II. by move/andP=> [] ->.
-- move => a l IH a0 a1. rewrite /= /IO_II. move/andP=> [] ->. intros. rewrite /=. 
-  unfold IO_II in IH. apply/IH. done. done.
-Qed.
+
 
 
 Lemma indep1 : forall l0 l1, indep (l0 ++ l1) -> if l1 is x::l1' then path IO_II x l1' else true.
@@ -684,6 +1011,14 @@ Inductive IO_seq : seq action -> Prop :=
  | IO_seq0 a b : IO a b ->  IO_seq ([::a; b])
  | IO_seq1 a b l : IO a b -> IO_seq (b::l) -> IO_seq (a::b::l).
 
+Lemma InDep_app : forall l0 l1, InDep (l0 ++ l1) -> 1 < size l1 -> InDep l1.
+Proof.
+elim. rewrite /=. done.
+move => a l IH l1. rewrite cat_cons. move => H. inversion H. subst.
+case : l H2 H IH.  rewrite /=. move => <-. done. 
+move => a0 l. rewrite cat_cons. case. move => <-. case : l.  case : l1. done. done. done. 
+intros. subst. rewrite H1 in H3. auto. 
+Qed.
 
 Lemma apply_InDep_app : forall l l0 l1 , InDep l -> l = l0++l1 -> 1 < size l1 -> InDep l1.
 Proof.
@@ -721,14 +1056,7 @@ Proof.
 intros.  apply : OutDep_app;auto. rewrite H0 in H. eauto. 
 Qed.
 
-Lemma delete_middle : forall a0 l0 a l1 a1 P, exists_depP (fun m => nth false m (size l0) = false) P a0 (l0 ++ a::l1) a1 ->
-                      exists_dep P a0 (l0++l1) a1.
-Proof.
-intros. move : H => [] m [] H0 [] H1 H2. exists ((take (size l0) m)++(drop (size l0).+1 m)).
-rewrite size_cat size_take size_drop H0 !size_cat /=. have : size l0 < size l0 + (size l1).+1 by lia.
-move => H3. rewrite H3. split. lia. split;auto. move : H1. rewrite !split_mask //=. rewrite H2 /= mask_cat //=. 
-by rewrite size_take H0 size_cat /= H3. 
-Qed.
+
 
 
 Lemma apply_linear : forall g s_tr a_p a0 s a1, Linear g -> Tr s_tr g -> s_tr = a_p++(a0::s++[::a1]) -> same_ch a0 a1 -> exists_dep InDep a0 s a1 /\ exists_dep OutDep a0 s a1.
@@ -736,22 +1064,8 @@ Proof.
 intros. rewrite H1 in H0. eauto. 
 Qed.
 
-Lemma get_neigbor : forall (P : action -> action -> bool) a p x_end m, path P a ((mask m p)++[::x_end]) -> exists x_in, x_in \in (a::p) /\ P x_in x_end. 
-Proof. 
-intros. 
-case : (split_list (mask m p)) H. move =>->. rewrite /= andbC /=. intros. exists a. by rewrite inE eqxx /=.
-move => [] l' [] a0 Heqa2.  move : (Heqa2) =>->. rewrite -catA. rewrite cat_path /=.
-move/andP=> [] _ /andP => [] [] _. rewrite andbC /=. move => HH.
-have : a0 \in a::p. rewrite inE.  apply/orP. right. apply (@mem_mask _ _  m). 
-rewrite Heqa2. by rewrite mem_cat inE eqxx orbC. 
-intros. exists a0. by rewrite x. 
-Qed.
 
-Lemma IO_II_in_action : forall a0 (l : label), IO_II a0 l -> in_action (ptcp_to a0) l.
-Proof.
-move => a0 a1. rewrite /IO_II. move/orP=>[]. rewrite /IO. move/eqP=>->. apply in_action_from.
-rewrite /II. move/eqP=>->. apply in_action_to.
-Qed.
+
 
 Lemma in_split : forall (A : eqType) l (x : A), x \in l -> exists l0 l1, l = l0 ++ x::l1.
 Proof.
